---
date: 2020-09-13
tags: 
  - stub
---

# Equality constraints (Haskell)

```hs
{-# LANGUAGE FlexibleContexts, TypeFamilies #-}
class Twice1 f where
  twice1 :: f -> f

class Twice2 f where
  twice2 :: f -> f

instance Twice1 (a -> a) where
  twice1 f = f . f

instance (a ~ b) => Twice2 (a -> b) where
  twice2 f = f . f
  
class Example a where
  transform :: Int -> a

instance Example Int where
  transform n = n + 1

instance Example Char where
  transform _ = 'x' 
  
apply1 x = twice1 transform x
apply2 x = twice2 transform x

apply1 :: (Example a, Twice1 (Int -> a)) => Int -> a
apply2 :: Int -> Int
```

For `apply1` we don't have sufficient information from transform's type (`Int -> a`) and the context.

For `apply2` we have information from the context, which asserts that `a ~ b`. Hence when `a ~ Int`, `b ~ Int`.

### Reference:

- [Infinite Negative utility - Haskell Type Equality Constraints](https://journal.infinitenegativeutility.com/haskell-type-equality-constraints)

