---
title: Writer Monad
date: "2020-06-21"
tags:
    - blog
    - Haskell
    - Monad
---

### Scenario

Imagine you have a function, `f` which takes in an argument `a`, produces a result `b`.

Now, you want log the input in the function.

In languages like Javascript where "functions" can produce side-effects, you could probably capture it in a state variable:

```js
let log = "" // We accumulate the logs here

function addOne (n) {
  log = log + `Adding one to ${n}`
  return n + 1
}
```

In haskell since functions have to be pure, you could do something like this:

```hs
type Log = String

addOne :: Int -> (Log, Int) // Embelishing the function to the accumulated log along with the result
addOne n = ("Adding one to " <> show n, n + 1)
```

Continuing on, let's invoke this function:

```hs
addedOne :: (Log, Int)
addedOne = addOne 1
```

Now suppose we want to use `addOne` on `addedOne` again. We have to lift `addOne`'s first argument into the `(,) Log` context..

```hs
addOne' :: (Log, Int) -> (Log, Int)
addOne' (log, n) = let (log2, n2) = addOne n
                   in (log ++ log2, n2)
```
*Notice the difference in the type signature for addOne and addOne'*

### Is there some way we can abstract some of this away?

If we observe `log ++ log2` it seems like a process we will repeat each time, combining `logs` whenever we call an adding function.

We also know the actual logic is in `addOne`, not `addOne'` which is a wrapper around `addOne`, allowing us to combine the `logs`.

By abstracting these patterns, we don't have to write boilerplate code to add the logs each time.

One abstraction we can have is a higher order function which can compose `addOne`s:

```hs
f :: (Int -> (Log, Int)) -> (Int -> (Log, Int)) -> (Int -> (Log, Int))
```

We can observe this resembles the "fish operator":

```hs
(>=>) :: Monad m => (a -> m b) -> (b -> m c) -> (a -> m c)
```

We can then try to implement a monadic type here:

```hs
data WriterL a = WriterL (Log, a)

class Monad WriterL where 
    return a = ("", a)
    f1 >=> f2 = \a -> let (l1, b) = f1 a
                          (l2, c) = f2 b
                      in  (l1 <> l2, c)
```

We can then use `>=>` to compose `addOne`s, composing the underlying functionality and combining the contexts, in this case the logs.

We do realize however, that `a -> m b` means that the composed function only looks at `a`.

As such, its treatment of the previous context in `m a` is fixed, when we defined the `>=>` operator. 
It monadically adds the logs.

Hence, we would not be able to `view/read` the logs along the way if we wanted to. The definition has made the `log` implicit.

Let's explore another construct to do `read`, the <8a11e368>.
