---
title: "What's the difference between Applicatives and Monads?"
date: "2020-06-21"
tags:
    - Applicatives
    - Monads
    - blog
---

# Monads

| Law            | definition `(>>=)`                         | definition `(>=>)`  | definition `join / j`    |
|----------------|--------------------------------------------|---------------------|--------------------------|
| left identity  | `return a >>= f = f a`                     | `return >=> g == g` | `join . return == id`    |
| right identity | `m >>= return = m`                         | `f >=> return == f` | `join . fmap pure == id` |
| associativity  | `(m >>= f) >>= g = m >>= (\x -> fx >>= g)` | `f >=> (g >=> h)`   | `j . fmap j = j . j`     |

# Applicatives

| Law          | definition                                     |
|--------------|------------------------------------------------|
| Identity     | `pure id <*> v = v`                            |
| Homomorphism | `pure f <*> pure x = pure (f x)`               |
| Interchange  | `u <*> pure y = pure ($ y) <*> u`              |
| Composition  | `pure (.) <*> u <*> v <*> w = u <*> (v <*> w)` |

# Differences

## What is the difference in `Applicatives` and `Monads`?


### High level understanding: 

key difference is in the second argument.

|                     | Monads `(>>=)`                                            | Applicatives `(<**>)`             |
| full type signature | `m a -> (a -> m b) -> m b`                                | `f a -> f (a -> b) -> f b`        |
| second argument     | `a -> m b`                                                | `f (a -> b)`                      |
| difference          | First argument, `a` can decide the future computation `m` | `a` is already in the context `f` |

### Examples for intuition


#### Error collecting

Monadic instance for Either:
``` hs
instance Monad (Either e) where
  return = Right
  v@(Left e) >>= _ = v
  Right a >>= f = f a
```

We observe that:
```hs
Left "Failed 0" >>= \_ -> Left "Failed 1" = Left "Failed 0"
```

We have lost the information: `Left "Failed 1"`

We might then be tempted to tweak the monad definition, to permit collecting error messages:

```hs
instance Monoid e => Monad (Either e) where
  return = Right
  Left e >>= f = ??
  Right a >>= f = f a
```

What do we want to do?
We want to apply f to a value: `f a`.
We can then pattern match on the result:

```hs
Left e >>= f = case f a of
  Left e' -> Left (e <> e')
  Right _ -> Left e
```

We realize that we can't do that however.
`Left e` is part of the context and does not return any result, 
in contrast to `Right a`.

Since `f` only takes in `a` as a functional dependency (since `f :: a -> m b`)
The context of the computation (`f a` in `f a -> (a -> m b)`) is opaque to it.

As such we can only do 2 things:

1) If we can get a result, pass it into f.
2) If we can't get a result, short circuit, since we can't evaluate f in any way.

Wait a minute, you say.

What if we did this:

```hs
Left e >>= \_ -> Left e' = Left (e <> e')
```

We can't do that either because we cannot go into function bodies! We can only see the mapping between input and the result.

What about this then!
```hs
Left e >> Left e = Left (e <> e')
```

Yes we could do that.

Note however, this is not powerful enough to give us a monad.

We are unable to define `(>>=)` in terms of `(>>)` (although the vice-versa works).

(Possible) Applicative instance for Either:
```hs
instance Monoid e => Applicative (Either e) where
  pure = Right
  Left e <*> Left e' = Left (e <> e')
  Left e <*> Right a = Right a
  Right f <*> Left e' = Left e'
  Right f <*> Right a = Right $ f a
```

This is because `Applicative` interface separate the context layer (`f (a -> b)`) rather than (`a -> f b`).

This makes the `(<*>)` operator able to work on the contexts as well.


#### Further examination of applicative patterns

Let's examine two types of computations:

Here, we can see that p1, p2 are not dependent on previous result.
The final result uses `return` which means it does not introduce any new context.
```hs
do val1 <- p1
   val2 <- p2
   return $ f val1 val2
```

We can thus represent this in applicative form:
```hs
pure f <*> val1 <*> val2
```

Here we can see a dependence:
```hs
do val1 <- p1
   val2 <- p2 val1 -- p2 is dependent on the result of p1
   return val2
```

Thus, this requires a monad.

### Closed under composition

m1 (m2 a) may or may not be a monad even if m1, m2 are monads.

a1 (a2 a) is an applicative as long as a1, a2 are applicatives.



References:
[Stack Overflow](https://stackoverflow.com/questions/23342184/difference-between-monad-and-applicative-in-haskell)
