---
title: Solving recurrence relations
date: "2020-08-10"
---

### Gain intuition and guess closed form solution
- Compute value of function at a few points
- Unfold recurrence a few steps

### Testing the hypothesis
- Try to prove by induction
- Use failed attempt to refine solution

### Example

$$\begin{split}
    T(n) &= 2T(n - 1) + 1
\end{split}$$

#### Compute value of function at a few points
Want to solve recurrence:

$$\begin{split}
    T(0) &= 0 \\
    T(n) &= 2T(n - 1) + 1
\end{split}$$

Compute a few steps:

$$\begin{split}
T(0) &= 0 \\
T(1) &= 2(T(0)) + 1 = 1 \\
T(2) &= 2(T(1)) + 1 = 3 \\
T(3) &= 2(T(2)) + 1 = 7 \\
T(4) &= 2(T(3)) + 1 = 15 \\
...
\end{split}$$

Hypothesis:

$$
T(n) = 2^n - 1
$$

Inductive proof:

Prove base case is true.

Show that if previous case is true: $T(n-1) = 2^(n - 1) - 1, current case $T(n) = 2^n - 1$.

$$\begin{split}
T(0) &= 0 = 2^0 - 1 \\
T(n) &= 2T(n - 1) + 1 \\
     &= 2(2^{n-1} - 1) + 1 \\
     &= 2^n - 1
\end{split}$$

#### Unroll recurrence

$$\begin{split}
T(n) &= 2T(n − 1) + 1 \\
     &= 2(2T(n − 2) + 1) + 1 = 4T(n − 2) + 3 \\
     &= 4(2T(n − 3) + 1) + 3 = 8T(n − 3) + 7 \\
     &= 16T(n − 4) + 15
\end{split}$$

Guess: $T(n) = 2^k T(n − k) + 2^k − 1 for 1 ≤ k ≤ n$

---

### Further examples
- [[fc20e943]]
- [[5ee769ab]]
- [[e5f376da]] 
