---
date: 2020-08-11
tags: 
  - induction
  - recurrence
---

# More recurrence induction examples

### Question

Assume $n = 2^{2^k}$ for some integer k.

Consider the following recurrence:

$$\begin{split}
    T(n) = \left\{ 
        \begin{array}l
            1,                       &if\ n = 2 \\
            \sqrt{n}T(\sqrt{n}) + n, &if\ n > 2
        \end{array}
\right.
\end{split}$$

On unfolding this recurrence, we get

$$\begin{split}
T(n) &= \sqrt{n} ( n^{1/4} T(n^{1/4}) ) + n       &= n^{3/4}T(n^{1/4}) + 2n \\
     &= n^{3/4}(n^{1/8}T(n^{1/8}) + n^{1/4}) + 2n &= n^{7/8}T(n^{1/8}) + 3n
\end{split}$$

Guess:

$$
    T(n) = n^{1 - 1/2^{i}}T(n^{1/2^i}) + i · n \ for \ 1 \leq i \leq k , n > 2 \ \ \ - \ (1)
$$

### Proof by induction

For i = 1:

$$\begin{split}
T(n) &= n^{1 - 1/2}T(n^{1/2}) + n \\
     &= n^{1/2}T(n^{1/2}) + n
\end{split}$$

For i = j:

$$
    T(n) = n^{1 - 1/2^{j}}T(n^{1/2^j}) + j · n
$$

Show for i = j + 1:

$$
    T(n) = n^{1 - 1/2^{j + 1}}T(n^{1/2^{j + 1}}) + (j + 1) · n
$$

Prove for i = j + 1:

$$\begin{split}
    T(n) &= n^{1 - 1/2^{j}}T(n^{1/2^j}) + j · n \\
         &= n^{1 - 1/2^{j}} · (n^{1/2^{j + 1}} T(n^{1/2^{j + 1}}) + n^{1/2^j}) + j · n \\
         &= n^{1 - 1/2^{j + 1}}T(n^{1/2^{j + 1}}) + n + j · n \\
         &= n^{1 - 1/2^{j + 1}}T(n^{1/2^{j + 1}}) + (j + 1) · n
\end{split}$$

Solve for:

$$\begin{split}
    n &= 2^{2^k} \\
    loglogn &= k
\end{split}$$

Substitute into (1):

$$\begin{split}
T(n) &= n^{1 - 1/2^{loglogn}}T(n^{1/2^{loglogn}}) + loglogn · n \\
     &= n^{1 - 1/logn}T(n^{1/logn}) + n\ log \log n \\
     &= \Theta(n\log \log n)
\end{split}$$
